lib/Word_Lib/Guide.thy
@@ -395,7 +395,7 @@ text \<open>
 
   \<^descr>[Changes since AFP 2024] ~
 
-    \<^item> Theory \<^text>\<open>Strict_part_mono\<close> is not part of text\<open>Word_Lib_Sumo\<close> any longer.
+    \<^item> Theory \<^text>\<open>Strict_part_mono\<close> is not part of \<^text>\<open>Word_Lib_Sumo\<close> any longer.
 
     \<^item> Session \<^text>\<open>Native_Word\<close>: Fact aliases \<^text>\<open>word_sdiv_def\<close> and \<^text>\<open>word_smod_def\<close>
       are gone, use \<^text>\<open>sdiv_word_def\<close> and \<^text>\<open>smod_word_def\<close> instead.
